More work

theories/Equiv/SimI.v
@@ -215,34 +215,212 @@ Qed.
 
 (** *** Fix Compatibility *)
 
-Lemma fix_compatible_separate t A (PR:ProofRelationI A) AL' AL F F' L L'
-  : (forall r,
+Lemma fix_compatible_separate t A (PR:ProofRelationI A) AL' AL F F'
+  : (forall r L L',
         labenv_sim t (sim r) PR (AL' ++ AL) (mapi I.mkBlock F ++ L) (mapi I.mkBlock F' ++ L')
         -> indexwise_r t (sim r) PR AL' F F' AL (mapi I.mkBlock F ++ L) (mapi I.mkBlock F' ++ L'))
     -> indexwise_paramrel PR F F' AL' AL
     -> separates PR AL' AL F F'
-    -> forall r, labenv_sim t (sim r) PR AL L L'
+    -> forall r L L', labenv_sim t (sim r) PR AL L L'
            -> indexwise_r t (sim r) PR AL' F F' AL (mapi I.mkBlock F ++ L) (mapi I.mkBlock F' ++ L').
 Proof.
-  intros ISIM LP SEP r SIML. pcofix CIH.
+  intros ISIM LP SEP r L L' SIML. pcofix CIH.
   eapply ISIM.
   eapply labenv_sim_extension'; eauto.
   eauto using indexwise_r_mon; eauto.
   eapply labenv_sim_mon; eauto.
 Qed.
 
+
+(*Require Import TraceEquiv.
+
+Definition pfx' (t:simtype) (σ σ':I.state) := forall L, prefix σ L -> prefix σ' L.
+Definition pfx
+           (r:rel3 simtype (fun _ : simtype => I.state) (fun (_ : simtype) (_ : I.state) => I.state))
+           (t:simtype) := pfx'.
+
+
+Inductive prefix_n {S} `{StateType S} : nat -> S -> list extevent -> Prop :=
+  | producesPrefixSilent n (σ:S) (σ':S) L :
+      step σ EvtTau σ'
+      -> prefix_n n σ' L
+      -> prefix_n (1+ n) σ L
+  | producesPrefixExtern n (σ:S) (σ':S) evt L :
+      activated σ
+      -> step σ evt σ'
+      -> prefix_n n σ' L
+      -> prefix_n (1+ n) σ (EEvtExtern evt::L)
+  | producesPrefixTerm n (σ:S) (σ':S) r
+    : result σ' = r
+      -> star2 step σ nil σ'
+      -> normal2 step σ'
+      -> prefix_n n σ (EEvtTerminate r::nil)
+  | producesPrefixPrefix n (σ:S)
+    : prefix_n n σ nil.
+
+Definition preincl n
+           {S} `{StateType S} {S'} `{StateType S'} (σ:S) (σ':S') :=
+  forall L,  prefix_n n σ L -> prefix σ' L.
+
+Lemma prefix_prefix_n {S} `{StateType S} σ L
+  : prefix σ L -> exists n, prefix_n n σ L.
+Proof.
+  intros P.
+  general induction P; try destruct IHP.
+  - exists (1+x). eauto 20 using @prefix_n.
+  - exists (1+x). eauto 20 using @prefix_n.
+  - exists 0. eauto 20 using @prefix_n.
+  - eexists 0. eauto 20 using @prefix_n.
+Qed.
+
+Lemma prefix_n_prefix {S} `{StateType S} σ L n
+  : prefix_n n σ L -> prefix σ L.
+Proof.
+  intros P.
+  general induction P; eauto using @prefix.
+Qed.
+
+Lemma preincl_prefix_incl {S} `{StateType S} {S'} `{StateType S'} (σ:S) (σ':S')
+  : (forall n, preincl n σ σ') -> forall L, prefix σ L -> prefix σ' L.
+Proof.
+  intros. eapply prefix_prefix_n in H2 as [? ?]. eapply H1; eauto.
+Qed.
+
+Definition pic n {S} `{StateType S} {S'} `{StateType S'}
+           (t:simtype) (σ:S) (σ':S') := preincl n σ σ'.
+
+Lemma pic_silent_step t n {S} `{StateType S} {S'} `{StateType S'} (σ1 σ1':S) (σ2 σ2':S')
+  : pic n t σ1' σ2'
+    -> step σ1 EvtTau σ1'
+    -> step σ2 EvtTau σ2'
+    -> pic (1+ n) t σ1 σ2.
+Proof.
+  intros. hnf; intros.
+  inv H4. relsimpl. eapply H1 in H7.
+  econstructor; eauto.
+  relsimpl. relsimpl.
+  assert (prefix_n n σ1' (EEvtTerminate (result σ') :: nil)) by eauto using @prefix_n.
+  eapply H1 in H5. econstructor; eauto.
+  econstructor. eauto. econstructor 4.
+Qed.
+
+Lemma labenv_sim_extension'' n t A (PR:ProofRelationI A) (AL AL':list A) F F' L L'
+  : indexwise_r t (pic n) PR AL' F F' AL (mapi I.mkBlock F ++ L) (mapi I.mkBlock F' ++ L')
+    -> indexwise_paramrel PR F F' AL' AL
+    -> separates PR AL' AL F F'
+    -> labenv_sim t (pic n) PR AL L L'
+    -> labenv_sim t (pic (S n)) PR (AL' ++ AL) (mapi I.mkBlock F ++ L) (mapi I.mkBlock F' ++ L').
+Proof.
+  intros SIM IPR [Len2 [Img [Ilt Ige]]] [Len1 [STL [STL' [PAR [IE LSIM]]]]].
+  hnf; do 5 (try split);
+    eauto 20 using smaller_I_mkBlocks, complete_paramrel, complete_indexes_exists with len.
+  intros f f' ? ? ? ? ? ? ? RN GetAL GetFL GetL'.
+  assert (Len3:❬AL'❭ = ❬mapi I.mkBlock F❭) by eauto with len.
+  eapply get_app_cases in GetFL. destruct GetFL as [GetFL'| [GetFL GE]].
+  - exploit Ilt; eauto. eapply get_range in GetFL'.
+    rewrite mapi_length in GetFL'; eauto.
+    eapply get_app_lt_1 in GetL'; [| rewrite mapi_length; eauto ].
+    inv_get. destruct x0 as [Z s], x as [Z' s']. simpl in *. clear EQ0 EQ.
+    eapply pic_silent_step; only 2-3: single_step.
+    simpl.
+    orewrite (f-f=0). orewrite (f'-f'=0). simpl.
+    exploit SIM; eauto.
+  - intros. exploit Ige; eauto. rewrite mapi_length in GE; eauto.
+    eapply get_app_right_ge in GetAL; [ | rewrite Len3; eauto ].
+    eapply get_app_right_ge in GetL'; [ | rewrite mapi_length; eauto ].
+    rewrite mapi_length in *.
+    eapply IndexRelDrop in RN; eauto; [| rewrite Len3; eauto].
+    exploit (LSIM (LabI  (f - ❬AL'❭)) (LabI (f' - Image AL'))) as SIMR; eauto.
+    rewrite Len3; eauto. rewrite Img; eauto.
+    eapply pic_silent_step; only 2-3: single_step.
+    Focus 2. eapply get_app_right; eauto. len_simpl. omega.
+    Focus 3. eapply get_app_right; eauto. len_simpl. omega.
+    simpl.
+    admit.
+    simpl; eauto with len. simpl; eauto with len.
+    (*eapply (@sim_Y_left I.state _ I.state _).
+    eapply (@sim_Y_right I.state _ I.state _).
+    rewrite Img in SIMR. rewrite Len3 in SIMR.
+    eapply paco3_mon; [| eauto].
+    eapply SIMR; eauto.
+    econstructor; simpl; eauto with len. simpl. eauto with len.
+    eapply I.StepGoto_mapi; simpl in *; eauto with len.
+    rewrite mapi_length. exploit STL; eauto. simpl in *. omega.
+    econstructor; simpl; eauto. simpl. eauto with len.
+    eapply I.StepGoto_mapi; simpl in *; eauto with len.
+    rewrite mapi_length. exploit STL'; eauto. simpl in *. omega.*)
+Admitted.
+
+Definition pic' {S} `{StateType S} {S'} `{StateType S'}
+           (t:simtype) (σ:S) (σ':S') := forall L, prefix σ L -> prefix σ' L.
+
+Lemma pic_pic' t A (PR:ProofRelationI A) AL' AL F F' L L'
+  : (forall n, (labenv_sim t (pic n) PR AL L L' -> indexwise_r t (pic n) PR AL' F F' AL L L'))
+    -> labenv_sim t pic' PR AL L L' -> indexwise_r t pic' PR AL' F F' AL L L'.
+Proof.
+  intros. hnf; intros.
+  hnf; intros.
+  eapply prefix_prefix_n in H6 as [? ?].
+  eapply H; eauto.
+  hnf; intros. edestruct H0. dcr.
+  split; eauto. split; eauto. split; eauto. split; eauto.
+  split; eauto. hnf; intros. hnf; intros.
+  eapply H14; eauto. eapply prefix_n_prefix; eauto.
+Qed.
+
+(*
+
+Lemma pic'_pic t A (PR:ProofRelationI A) AL' AL F F' L L'
+  : (labenv_sim t pic' PR AL L L' -> indexwise_r t pic' PR AL' F F' AL L L')
+    -> (forall n, (labenv_sim t (pic n) PR AL L L' -> indexwise_r t (pic n) PR AL' F F' AL L L')).
+Proof.
+  intros. hnf; intros.
+  hnf; intros.
+  eapply prefix_n_prefix in H6.
+  eapply H; eauto.
+  hnf; intros. edestruct H0. dcr.
+  split; eauto. split; eauto. split; eauto. split; eauto.
+  split; eauto. hnf; intros. hnf; intros.
+  eapply H14; eauto. eapply prefix_prefix_n in H22 as [? ?]. eauto.
+Qed.
+*)
+
+
+
+Lemma fix_compatible_separate' t A (PR:ProofRelationI A) AL' AL F F' L L'
+  : (forall n, (labenv_sim t (pic n) PR (AL' ++ AL) (mapi I.mkBlock F ++ L) (mapi I.mkBlock F' ++ L')
+           -> indexwise_r t (pic n) PR AL' F F' AL (mapi I.mkBlock F ++ L) (mapi I.mkBlock F' ++ L')))
+    -> indexwise_paramrel PR F F' AL' AL
+    -> separates PR AL' AL F F'
+    -> (forall n, labenv_sim t (pic n) PR AL L L'
+    -> indexwise_r t (pic n) PR AL' F F' AL (mapi I.mkBlock F ++ L) (mapi I.mkBlock F' ++ L')).
+Proof.
+  intros ISIM LP SEP k SIML. general induction k.
+  - intros. hnf; intros. hnf; intros.
+    inv H4; eauto using @prefix.
+    eapply ISIM; eauto using @prefix.
+    admit.
+  - eapply ISIM; eauto.
+    eapply labenv_sim_extension''; eauto.
+    Focus 2.
+    eapply labenv_sim_mon; eauto. admit.
+    eapply IHk; eauto.
+    eapply labenv_sim_mon; eauto. admit.
+Admitted.
+ *)
+
 (** *** Extension Lemma *)
 
-Lemma labenv_sim_extension t A (PR:ProofRelationI A) (AL AL':list A) F F' L L'
-  : (forall r,
+Lemma labenv_sim_extension t A (PR:ProofRelationI A) (AL AL':list A) F F'
+  : (forall r L L',
         labenv_sim t (sim r) PR (AL' ++ AL) (mapi I.mkBlock F ++ L) (mapi I.mkBlock F' ++ L')
         -> indexwise_r t (sim r) PR AL' F F' AL (mapi I.mkBlock F ++ L) (mapi I.mkBlock F' ++ L'))
     -> indexwise_paramrel PR F F' AL' AL
     -> separates PR AL' AL F F'
-    -> forall r, labenv_sim t (sim r) PR AL L L'
+    -> forall r L L', labenv_sim t (sim r) PR AL L L'
         -> labenv_sim t (sim r) PR (AL' ++ AL) (mapi I.mkBlock F ++ L) (mapi I.mkBlock F' ++ L').
 Proof.
-  intros ISIM IP SEP r SIML.
+  intros ISIM IP SEP r L L' SIML.
   eapply labenv_sim_extension'; eauto.
   eapply indexwise_r_mon.
   eapply fix_compatible_separate; eauto. eauto.
@@ -250,6 +428,7 @@ Qed.
 
 (** *** Fun Compatibility *)
 
+(*
 Lemma sim_fun t A (PR:ProofRelationI A) (AL AL':list A) F F' L L' V V' s s'
   : (forall r, labenv_sim t (sim r) PR (AL' ++ AL) (mapi I.mkBlock F ++ L) (mapi I.mkBlock F' ++ L')
           -> (sim r \3/ r) t (mapi I.mkBlock F ++ L, V, s) (mapi I.mkBlock F' ++ L', V', s'))
@@ -266,6 +445,7 @@ Proof.
   eapply SIM_s.
   eapply labenv_sim_extension; eauto.
 Qed.
+ *)
 
 (** *** Specialized Version if function bindings are not changed *)
 
@@ -306,17 +486,17 @@ Qed.
 
 Hint Resolve IndexRelIP_refl.
 
-Lemma labenv_sim_extension_ptw t A (PR:PointwiseProofRelationI A) (AL AL':list A) F F' L L'
-  : (forall r ,
+Lemma labenv_sim_extension_ptw t A (PR:PointwiseProofRelationI A) (AL AL':list A) F F'
+  : (forall r L L',
         labenv_sim t (sim r) PR (AL' ++ AL) (mapi I.mkBlock F ++ L) (mapi I.mkBlock F' ++ L')
         -> indexwise_r t (sim r) PR AL' F F' AL (mapi I.mkBlock F ++ L) (mapi I.mkBlock F' ++ L'))
     -> indexwise_paramrel PR F F' AL' AL
     -> length AL' = length F
     -> length F = length F'
-    -> forall r, labenv_sim t (sim r) PR AL L L'
+    -> forall r L L', labenv_sim t (sim r) PR AL L L'
         -> labenv_sim t (sim r) PR (AL' ++ AL) (mapi I.mkBlock F ++ L) (mapi I.mkBlock F' ++ L').
 Proof.
-  intros ISIM IP Len1 Len2 r SIML.
+  intros ISIM IP Len1 Len2 r L L' SIML.
   assert (separates PR AL' AL F F'). {
     destruct SIML; dcr.
     hnf; destruct PR; simpl; repeat split; intros; omega.
@@ -326,19 +506,19 @@ Proof.
   eapply fix_compatible_separate; eauto. eauto.
 Qed.
 
-Lemma sim_fun_ptw t A (PR:PointwiseProofRelationI A) (AL AL':list A) F F' L L' V V' s s'
-  : (forall r, labenv_sim t (sim r) PR (AL' ++ AL) (mapi I.mkBlock F ++ L) (mapi I.mkBlock F' ++ L')
+Lemma sim_fun_ptw t A (PR:PointwiseProofRelationI A) (AL AL':list A) F F' V V' s s'
+  : (forall r L L', labenv_sim t (sim r) PR (AL' ++ AL) (mapi I.mkBlock F ++ L) (mapi I.mkBlock F' ++ L')
           -> (sim r \3/ r) t (mapi I.mkBlock F ++ L, V, s) (mapi I.mkBlock F' ++ L', V', s'))
-    -> (forall r,
+    -> (forall r L L',
           labenv_sim t (sim r) PR (AL' ++ AL) (mapi I.mkBlock F ++ L) (mapi I.mkBlock F' ++ L')
           -> indexwise_r t (sim r) PR AL' F F' AL (mapi I.mkBlock F ++ L) (mapi I.mkBlock F' ++ L'))
     -> indexwise_paramrel PR F F' AL' AL
     -> length AL' = length F
     -> length F = length F'
-    -> forall r, labenv_sim t (sim r) PR AL L L'
+    -> forall r L L', labenv_sim t (sim r) PR AL L L'
            -> sim r t (L, V, stmtFun F s) (L', V', stmtFun F' s').
 Proof.
-  intros SIM_s ISIM IP Len1 Len2 r SIML.
+  intros SIM_s ISIM IP Len1 Len2 r L L' SIML.
   pone_step.
   eapply SIM_s.
   eapply labenv_sim_extension_ptw; eauto.
@@ -444,3 +624,382 @@ Proof.
       * stuck. inv H2. simpl in *. inv def. simpl in *. inv_get.
       * stuck. inv H2. simpl in *. inv def. simpl in *. inv_get.
 Qed.
+
+
+Definition trivs (f:external) :=
+  stmtLet default_var (Call f nil) (stmtReturn (Con default_val)).
+
+Definition trivL (b:I.block) (f:external) :=
+  match b with
+  | I.blockI Z s n => I.blockI Z (trivs f) n
+  end.
+
+Lemma triv_sat t A (PR:PointwiseProofRelationI A) AL L L' XF r (Len:❬XF❭= ❬L❭) (Len2:❬L❭=❬L'❭)
+  : labenv_sim t (sim r) PR AL L L'
+    -> labenv_sim t (sim bot3) PR AL (trivL ⊜ L XF) (trivL ⊜ L' XF).
+Proof.
+  intros. hnf; intros.
+  destruct H; dcr. len_simpl.
+  split; eauto.
+  split. {
+    hnf; intros; inv_get. destruct x; simpl. exploit H1; eauto.
+  }
+  split. {
+    hnf; intros; inv_get. destruct x; simpl. exploit H3; eauto.
+  }
+  split. {
+    hnf; intros; inv_get. destruct x,x1; simpl in *; clear_trivial_eqs.
+    exploit H2; eauto.
+  }
+  split. hnf; intros; inv_get. edestruct H4; eauto. inv_get.
+  eexists; eapply zip_get; eauto.
+  hnf; intros. pone_step. inv_get. simpl.
+  destruct x,x1; simpl in *; clear_trivial_eqs. unfold trivs.
+  assert (f=f'). hnf in H0. destruct PR. simpl in *. destruct f, f'; simpl in *. congruence.
+  rewrite H15. subst. inv_get.
+  left. pextern_step; eauto.
+  hnf; intros. eexists; eauto. eexists. econstructor. simpl. reflexivity.
+  hnf; intros. eexists; eauto. eexists. econstructor. simpl. reflexivity.
+  left. pno_step.
+  left. pno_step.
+  Grab Existential Variables.
+  eapply default_val.
+  eapply default_val.
+Qed.
+
+Require Import Sawtooth.
+
+Lemma drop_le n X (L L':list X)
+      (LE:n <= ❬L❭)
+  : drop n (L ++ L') = drop n L ++ L'.
+Proof.
+  general induction L; simpl in *.
+  - invc LE. reflexivity.
+  - destruct n; simpl; eauto.
+    rewrite IHL; eauto. omega.
+Qed.
+
+Lemma drop_app n X (L L':list X)
+  : drop n (L ++ L') = drop n L ++ drop (n - ❬L❭) L'.
+Proof.
+  general induction L; simpl in *.
+  - rewrite drop_nil. orewrite (n - 0 = n). reflexivity.
+  - destruct n; simpl; eauto.
+Qed.
+
+Lemma trivL_step_tau_inv (L1:〔I.block〕) L XF E s σ
+  : step (L1 ++ trivL ⊜ L XF, E, s) EvtTau σ
+    -> (exists k L2 E' s', σ = (drop k (L2 ++ L1 ++ trivL ⊜ L XF), E', s') /\
+                     step (L1 ++ L, E, s) EvtTau (drop k (L2 ++ L1 ++ L), E', s')
+                     /\ k <= ❬L1❭ + ❬L2❭)
+      \/ exists f Y, s = stmtApp f Y /\ f >= ❬L1❭.
+Proof.
+  intros.
+  inv H;
+    try now (left; eexists 0, nil; do 2 eexists; (split; [try reflexivity|split;[try single_step|simpl; omega]])).
+  - eapply get_app_cases in Ldef as [|[? ?]].
+    + left. eexists (l - I.block_n blk), nil.
+      do 2 eexists; (split; [try reflexivity|split;[try single_step|simpl; try omega]]).
+      simpl. eauto using get_app.
+      eapply get_range in H0. omega.
+    + right. eauto.
+  - left. eexists 0, (mapi I.mkBlock s0). simpl.
+    do 2 eexists; (split; [try reflexivity|split;[try single_step|simpl; try omega]]).
+Qed.
+
+Definition externalsE (e:exp) :=
+  match e with
+  | Operation _ => {}
+  | Call f _ => singleton f
+  end.
+
+Fixpoint externals (s:stmt) : set var :=
+  match s with
+  | stmtLet x e s0 => externalsE e ∪ externals s0
+  | stmtIf e s1 s2 => externals s1 ∪ externals s2
+  | stmtApp l Y => {}
+  | stmtReturn e => {}
+  | stmtFun F t => list_union ((fun Zs => externals (snd Zs)) ⊝ F) ∪ externals t
+  end.
+
+Definition bexternals (b:I.block) :=
+  externals (I.block_s b).
+
+Lemma trivL_step_tau_inv' (L1:〔I.block〕) L XF E s σ (STL:sawtooth (L1 ++ L))
+      (DISJ:disj (of_list XF) (externals s ∪ list_union (bexternals ⊝ L1)))
+  : step (L1 ++ trivL ⊜ L XF, E, s) EvtTau σ
+    -> (exists L2 E' s', σ = (L2 ++ trivL ⊜ L XF, E', s') /\
+                   step (L1 ++ L, E, s) EvtTau (L2 ++ L, E', s') /\ sawtooth (L2 ++ L) /\
+                   disj (of_list XF) (externals s' ∪ list_union (bexternals ⊝ L2)))
+      \/ exists f Y vl Z n s' xf, s = stmtApp f Y /\ f >= ❬L1❭ /\
+                      omap (op_eval E) Y = Some vl /\
+                      get XF (f - ❬L1❭) xf  /\
+                      get L (f - ❬L1❭) (I.blockI Z s' n) /\
+                 σ = (drop ((f - ❬L1❭)- n) (trivL ⊜ L XF), E[Z <-- Some ⊝ vl], trivs xf) /\
+                 step (L1 ++ L, E, s) EvtTau (drop ((f - ❬L1❭) - n) L, E[Z <-- Some ⊝ vl], s').
+Proof.
+  intros.
+  inv H; simpl in *;
+    try now (
+          left; eexists L1; do 2 eexists;
+          (split; [try reflexivity
+                  |split; [try single_step
+                          |split; [eassumption|eapply disj_2_incl; eauto with cset]]])
+        ).
+  - eapply get_app_cases in Ldef as [|[? ?]].
+    + left. eexists (drop (l - I.block_n blk) L1).
+      rewrite <- !drop_le; eauto.
+      do 2 eexists; (split; [try reflexivity|split; try single_step]).
+      eapply get_app; eauto.
+      split.
+      eapply sawtooth_drop'; eauto using get_app.
+      rewrite drop_map. rewrite list_union_drop_incl.
+      eapply disj_2_incl; eauto.
+      eapply union_incl_split; eauto with cset.
+      rewrite <- incl_list_union; eauto using map_get_1; try reflexivity.
+      cset_tac.
+      eapply get_range in H0. omega.
+      eapply get_range in H0. omega.
+    + right.
+      inv_get. destruct x as [Z s' n].
+      do 7 eexists; split; eauto.
+      split; eauto.
+      split; eauto.
+      split; eauto.
+      split; eauto. simpl.
+      rewrite drop_app_gen.
+      admit. admit.
+  - left. eexists (mapi I.mkBlock s0 ++ L1). rewrite <- !app_assoc.
+    do 2 eexists; (split; [try reflexivity|try single_step]).
+Admitted.
+
+
+Lemma trivs_star_inv (L:〔I.block〕) E xf σ n
+  :  star2n step n (L, E, trivs xf) nil σ
+     -> n = 0 /\ σ = (L, E, trivs xf).
+Proof.
+  intros. inv H; eauto.
+  exfalso. inv H1. isabsurd.
+Qed.
+
+Lemma trivL_plus_step_tau_inv L1 (L:〔I.block〕) XF E s σ n
+      (STEP:star2n step n (L1 ++ trivL ⊜ L XF, E, s) nil σ) (STL:sawtooth (L1 ++ L))
+      (DISJ:disj (of_list XF) (externals s ∪ list_union (bexternals ⊝ L1)))
+  : ((exists σ' L2 E' s',
+         star2n step n (L1 ++ L, E, s) nil σ' /\
+         sawtooth (L2 ++ L) /\ σ = (L2 ++ trivL ⊜ L XF, E', s') /\
+         σ' = (L2 ++ L, E', s') /\
+         disj (of_list XF) (externals s' ∪ list_union (bexternals ⊝ L2)))
+     \/ ( exists σ' E' f Y vl Z n' s' xf,
+           star2n step n (L1 ++ L, E, s) nil σ' /\
+           omap (op_eval E') Y = Some vl /\
+           get XF f xf  /\
+           get L f (I.blockI Z s' n') /\
+           σ = (drop (f - n') (trivL ⊜ L XF), E'[Z <-- Some ⊝ vl], trivs xf) /\
+           σ' = (drop (f - n') L, E'[Z <-- Some ⊝ vl], s'))).
+Proof.
+  intros. general induction STEP.
+  - left.
+    eexists.
+    eexists L1; do 2 eexists; eauto 20 using star2n.
+  - destruct y, yl; isabsurd.
+    edestruct trivL_step_tau_inv'; eauto.
+    + dcr. subst. simpl in *; clear_trivial_eqs.
+      exploit IHSTEP as IH; eauto.
+      destruct IH as [[? ?]|[? ?]]; dcr; subst.
+      * left. do 4 eexists. split.
+        -- eapply S_star2n with (y:=EvtTau) (yl:=nil); eauto.
+        -- eauto.
+      * right.
+        do 9 eexists. split.
+        -- eapply S_star2n with (y:=EvtTau) (yl:=nil); eauto.
+        -- eauto.
+    + destruct H0; dcr; subst.
+      edestruct trivs_star_inv; eauto; subst.
+      right.
+      do 9 eexists. split.
+      * eapply S_star2n with (y:=EvtTau) (yl:=nil); eauto.
+        econstructor.
+      * eauto.
+Qed.
+
+Lemma normal2_labenv_I E s (L L':I.labenv)
+  : normal2 step (L, E, s)
+    -> (forall n b b', get L n b -> get L' n b' -> block_Z b = block_Z b')
+    -> ❬L'❭ = ❬L❭
+    -> normal2 step (L', E, s).
+Proof.
+  intros. hnf; intros. eapply H.
+  destruct H2 as [? [? ?]].
+  eexists x.
+  inv H2; simpl in *; inv_get; eexists; try single_step.
+  econstructor; eauto. exploit H0; eauto. rewrite H4. eauto.
+Qed.
+
+Lemma event_inversion t (L:I.labenv) E xf L' E' s'
+  : (forall evt σ1'', step (L, E, trivs xf) evt σ1'' -> exists σ2'',
+          step (L', E', s') evt σ2'' /\ sim bot3 t σ1'' σ2'')
+    -> exists x s'', s' = stmtLet x (Call xf nil) s''.
+Proof.
+  intros.
+  edestruct H.
+  - hnf. eapply I.StepExtern with (v:=default_val). reflexivity.
+  - dcr. inv H1. destruct Y; simpl in *; eauto.
+    monad_inv def.
+Qed.
+
+
+Lemma trivs_inversion (L:I.labenv) XF E s L' E' xf n s' x L2
+      (GET:get XF n xf) (Len:❬XF❭ = ❬L❭) (ND:NoDupA eq XF)
+      (NOTIN1:xf ∉ externals s) (NOTIN2:xf ∉ list_union (bexternals ⊝ L2))
+  (Step:step (L2 ++ trivL ⊜ L XF, E, s) EvtTau (L', E', stmtLet x (Call xf nil) s'))
+  : exists Y b vl, s = stmtApp (LabI (❬L2❭ + n)) Y
+         /\ get L n b
+         /\ ❬Y❭ = ❬I.block_Z b❭
+         /\ omap (op_eval E) Y = Some vl.
+Proof.
+  inv Step; simpl in *;
+    try now (exfalso; cset_tac).
+  eapply get_app_cases in Ldef as [?|[? ?]].
+  - exfalso. eapply NOTIN2. rewrite <- incl_list_union; eauto using map_get_1; try reflexivity.
+    unfold bexternals. rewrite H5. simpl. cset_tac.
+  - destruct blk; simpl in *. subst.
+    inv_get. destruct x0. simpl in *. unfold trivs in EQ. invc EQ.
+    decide (n = l - ❬L2❭).
+    + rewrite e. do 3 eexists.
+      split. f_equal. destruct l. f_equal. simpl in *. omega.
+      eauto.
+    + exfalso.
+      eapply NoDupA_get_neq in GET; eauto. congruence.
+Qed.
+
+Lemma star2n_trans_silent (X : Type) (R : X -> event -> X -> Prop) n m x y z
+  : star2n R n x nil y
+    -> star2n R m y nil z
+    -> star2n R (n + m) x nil z.
+Proof.
+  intros A B.
+  general induction A; simpl; eauto.
+  econstructor; eauto.
+  destruct y, yl; isabsurd.
+  eapply IHA; eauto.
+Qed.
+
+Lemma star2n_decomp_right (X : Type) (R : X -> event -> X -> Prop) n x y
+  : star2n R (S n) x nil y
+    -> exists z, star2n R n x nil z /\ R z EvtTau y.
+Proof.
+  general induction n.
+  - repeat invtc star2n.
+    destruct y0; isabsurd.
+    eauto using star2n.
+  - invtc star2n.
+    destruct y0, yl; isabsurd.
+    eapply IHn in H4; dcr.
+    eauto using star2n.
+Qed.
+
+Lemma labenv_lift r t A (PR:PointwiseProofRelationI A) XF AL L1 L2 L L' E E' s s'
+      (Len:❬XF❭=❬L❭) (Len2:❬L❭=❬L'❭)
+      (DISJ:disj (of_list XF) (externals s ∪ list_union (bexternals ⊝ L1)))
+      (DISJ':disj (of_list XF) (externals s' ∪ list_union (bexternals ⊝ L2)))
+  (LAB:labenv_sim t (sim r) PR AL L L')
+  (SIMbot:sim bot3 t (L1 ++ trivL ⊜ L XF, E, s) (L2 ++ trivL ⊜ L' XF, E', s'))
+  (STL1:sawtooth (L1 ++ L))
+  (STL2: sawtooth (L2 ++ L'))
+  : sim r t (L1 ++ L, E, s) (L2 ++ L', E', s').
+Proof.
+  revert_all. pcofix CIH; intros.
+  pinversion SIMbot; subst.
+  - eapply plus2_star2n in H. eapply plus2_star2n in H0. dcr.
+    edestruct (trivL_plus_step_tau_inv _ _ _ H2); eauto. dcr.
+    destruct H4; dcr; subst.
+    + edestruct (trivL_plus_step_tau_inv _ _ _ H0); eauto. dcr.
+      destruct H6; dcr; subst.
+      * eapply star2n_plus2 in H3.
+        eapply star2n_plus2 in H4.
+        pfold.
+        econstructor 1; eauto.
+      * eapply star2n_plus2 in H4.
+        eapply sim_activated in H1 as [? [? [? ?]]]; dcr.
+        destruct x1 as [[? ?] ?].
+        eapply event_inversion in H11 as [? [? ?]]. subst. clear H12.
+        eapply star2_star2n in H. dcr.
+        eapply star2n_trans_silent in H10; eauto. simpl in *.
+        eapply trivL_plus_step_tau_inv in H10 as [? [? ?]]; eauto.
+        destruct H10.
+        exfalso; dcr. subst. invc H11. simpl in *.
+        eapply H15. eapply get_in_of_list; eauto.
+        clear. cset_tac. dcr. subst. invc H14. inv_get.
+        eapply star2n_star2 in H.
+        eapply plus2_star2 in H4.
+        admit.
+        -- hnf. do 2 eexists; econstructor. reflexivity.
+    + admit.
+  - admit.
+  - eapply star2_star2n in H0. dcr.
+    edestruct (trivL_plus_step_tau_inv _ _ _ H2); eauto. dcr.
+    destruct H4; dcr; subst.
+    + eapply star2n_star2 in H3.
+      pfold.
+      eapply SimErr; try eapply H3; eauto.
+      eapply normal2_labenv_I; eauto with len.
+      clear. intros.
+      eapply get_app_cases in H as [?|[? ?]]; inv_get; eauto.
+      eapply get_app_ge in H0; eauto.
+      destruct x; inv_get; reflexivity.
+    + exfalso. eapply H1.
+      hnf. do 2 eexists. econstructor. reflexivity.
+  - eapply star2_star2n in H0. eapply star2_star2n in H1. dcr.
+    edestruct (trivL_plus_step_tau_inv _ _ _ H4); eauto. dcr.
+    edestruct (trivL_plus_step_tau_inv _ _ _ H1); eauto. dcr.
+    pfold.
+    eapply star2n_star2 in H5. eapply star2n_star2 in H7.
+    destruct H6; dcr; subst.
+    + destruct H8; dcr; subst.
+      * eapply SimTerm; try eapply H5; try eapply H7; eauto.
+        eapply normal2_labenv_I; eauto with len.
+        clear. intros.
+        eapply get_app_cases in H as [?|[? ?]]; inv_get; eauto.
+        eapply get_app_ge in H0; eauto.
+        destruct x; inv_get; reflexivity.
+        eapply normal2_labenv_I; eauto.
+        clear. intros.
+        eapply get_app_cases in H as [?|[? ?]]; inv_get; eauto.
+        eapply get_app_ge in H0; eauto.
+        destruct x; inv_get; reflexivity.
+        len_simpl. rewrite Len. rewrite min_l; eauto.
+        omega.
+      * exfalso. eapply H2.
+        hnf. do 2 eexists. econstructor. reflexivity.
+    + exfalso. eapply H3.
+      hnf. do 2 eexists. econstructor. reflexivity.
+Qed.
+
+
+Lemma key t A (PR:PointwiseProofRelationI A) AL' AL F F'
+  : (forall L L', ❬L❭=❬L'❭ -> labenv_sim t (sim bot3) PR AL L L' -> indexwise_r t (sim bot3) PR AL' F F' AL L L')
+    -> (forall r L L', ❬L❭=❬L'❭-> (labenv_sim t (sim r) PR AL L L' -> indexwise_r t (sim r) PR AL' F F' AL L L')).
+Proof.
+  intros. hnf; intros.
+  assert (XFE:exists XF:list external, ❬XF❭ = ❬L❭) by admit.
+  destruct XFE as [XF XFlen].
+  exploit (H (trivL ⊜ L XF) (trivL ⊜ L' XF)).
+  eauto with len.
+  eapply (triv_sat PR XF XFlen H0 H1); eauto.
+  exploit H7; eauto.
+  eapply labenv_lift with (L1:=nil) (L2:=nil); eauto.
+Qed.
+  clear H.
+
+(*
+  hnf; intros.
+  eapply prefix_n_prefix in H6.
+  eapply H; eauto.
+  hnf; intros. edestruct H0. dcr.
+  split; eauto. split; eauto. split; eauto. split; eauto.
+  split; eauto. hnf; intros. hnf; intros.
+  eapply H14; eauto. eapply prefix_prefix_n in H22 as [? ?]. eauto.
+Qed.
+ *)
+Admitted.
